NewMain.thy
@@ -2,16 +2,16 @@ theory NewMain
 imports Main NewOCL NewSQL NewOCLtoSQL
 begin
 
-theorem "OCL2PSQL (eval (SINGLE (OCLNatLiteralExp i)) om) = exec (SELECT (SQLNatSelItem i)) om"
+theorem "OCL2PSQL (eval (SINGLETYPE (OCLNatLiteralExp i)) om) = exec (SELECT (SQLNatSelItem i)) om"
 by auto
 
-theorem "OCL2PSQL (eval (SINGLE (OCLStringLiteralExp s)) om) = exec (SELECT (SQLStringSelItem s)) om"
+theorem "OCL2PSQL (eval (SINGLETYPE (OCLStringLiteralExp s)) om) = exec (SELECT (SQLStringSelItem s)) om"
 by auto
 
-theorem "OCL2PSQL (eval (SINGLE (OCLBoolLiteralExp b)) om) = exec (SELECT (SQLBoolSelItem b)) om"
+theorem "OCL2PSQL (eval (SINGLETYPE (OCLBoolLiteralExp b)) om) = exec (SELECT (SQLBoolSelItem b)) om"
 by auto
 
-theorem "OCL2PSQL (eval (COL (OCLAllInstancesExp NewOCL.PERSON)) om) = exec (SELECTFROM (SQLColSelItem (PCol ID)) (NewSQL.PERSON)) om"
+theorem "OCL2PSQL (eval (COLLECTIONTYPE (OCLAllInstancesExp NewOCL.PERSON)) om) = exec (SELECTFROM (SQLColSelItem (PCol ID)) (NewSQL.PERSON)) om"
 proof (induct om)
 case (OBJECTMODEL ps es)
 then show ?case 
@@ -24,7 +24,7 @@ next
 qed
 qed
 
-theorem "OCL2PSQL (eval (SINGLE (OCLSizeExp (OCLAllInstancesExp NewOCL.PERSON))) om) = exec (SELECTFROM (SQLCount (PCol ID)) (NewSQL.PERSON)) om"
+theorem "OCL2PSQL (eval (SINGLETYPE (OCLSizeExp (OCLAllInstancesExp NewOCL.PERSON))) om) = exec (SELECTFROM (SQLCount (PCol ID)) (NewSQL.PERSON)) om"
 proof (induct om)
 case (OBJECTMODEL ps es)
 then show ?case 
@@ -37,7 +37,7 @@ next
 qed
 qed
 
-theorem "OCL2PSQL (eval (SINGLE (OCLIsEmptyExp (OCLAllInstancesExp NewOCL.PERSON))) om) = exec (SELECTFROM (SQLEq (SQLCount (PCol ID)) (SQLNatSelItem 0)) (NewSQL.PERSON)) om"
+theorem "OCL2PSQL (eval (SINGLETYPE (OCLIsEmptyExp (OCLAllInstancesExp NewOCL.PERSON))) om) = exec (SELECTFROM (SQLEq (SQLCount (PCol ID)) (SQLNatSelItem 0)) (NewSQL.PERSON)) om"
 proof (induct om)
 case (OBJECTMODEL ps es)
 then show ?case 
@@ -50,7 +50,7 @@ next
 qed
 qed
 
-theorem "OCL2PSQL (eval (SINGLE (OCLIsNotEmptyExp (OCLAllInstancesExp NewOCL.PERSON))) om) = exec (SELECTFROM (SQLNotEq (SQLCount (PCol ID)) (SQLNatSelItem 0)) (NewSQL.PERSON)) om"
+theorem "OCL2PSQL (eval (SINGLETYPE (OCLIsNotEmptyExp (OCLAllInstancesExp NewOCL.PERSON))) om) = exec (SELECTFROM (SQLNotEq (SQLCount (PCol ID)) (SQLNatSelItem 0)) (NewSQL.PERSON)) om"
 proof (induct om)
 case (OBJECTMODEL ps es)
 then show ?case 
